theories/oneshot.v
@@ -1,0 +1,32 @@
+From iris.algebra Require Import agree excl csum updates.
+
+Definition oneshot A := csum (excl unit) (agree A).
+Canonical Structure oneshotR (A: ofeT) := csumR (exclR unitC) (agreeR A).
+Definition unset {A: ofeT}: oneshotR A := Cinl (Excl ()).
+Definition agreed {A: ofeT} (x: A): oneshotR A := Cinr (to_agree x).
+
+Section Facts.
+  Context {A: ofeT}.
+
+  Global Instance agreed_ne: NonExpansive (@agreed A).
+  Proof. solve_proper. Qed.
+
+  Global Instance unset_exclusive: Exclusive (@unset A).
+  Proof. apply _. Qed.
+
+  Global Instance agreed_persistent (x: A): Persistent (agreed x).
+  Proof. apply _. Qed.
+  
+  Lemma oneshot_update (x: A): unset ~~> agreed x.
+  Proof. by apply cmra_update_exclusive. Qed.
+
+  Lemma agreed_valid (x y: A): ✓(agreed x ⋅ agreed y) → x ≡ y.
+  Proof.
+    rewrite /agreed Cinr_op.
+    apply agree_op_inv'.
+  Qed.
+
+  Context `{Discrete A}.
+  Global Instance oneshot_discrete: CMRADiscrete (oneshotR A).
+  Proof. apply _. Qed.
+End Facts.
