theories/typetranslation.v
@@ -1,0 +1,273 @@
+From iris.proofmode Require Import tactics classes.
+From iris.base_logic.lib Require Import invariants own.
+From iris.algebra Require Import updates agree big_op.
+From esop Require Import types oneshot specification corecalculus.
+From stdpp Require Import gmap coPset.
+
+Module TypeTranslation(AxSem: AxiomaticSemantics).
+  Module Import Axiomatics := AxSem <+ AxiomaticFacts.
+  Variant name_entry := Loc (l: loc) | Task (t: tid) (γ: gname).
+  Definition name_map := gmap gname name_entry.
+  Variant conn_name := RET | name (ξ: gname) | var (x: string).
+  Instance: EqDecision conn_name.
+  Proof. solve_decision. Defined.
+  Instance: Countable conn_name :=
+    Build_Countable conn_name _
+      (λ c, match c with RET => 1 | name ξ => ξ~0 | var x => (encode x)~1 end)%positive
+      (λ p, match p with 1 => Some RET | ξ~0 => Some (name ξ) | x~1 => var <$> decode x end)%positive
+      _.
+  Proof.
+    destruct x; auto.
+    rewrite decode_encode; done.
+  Qed.
+  
+  Definition conn_map := gmap conn_name val.
+  Coercion VConst: const >-> val.
+  Coercion of_gset: gset >-> coPset.
+  
+  Definition int_type {Σ} := val → name_map → val → iProp Σ.
+  Definition int_heap {Σ} := conn_map → name_map → iProp Σ.
+
+  Definition overlap `{Countable K,Collection K C} (s: C) {A} (m m': gmap K A) :=
+    ∀ k, k ∈ s → m!!k = m'!!k.
+  Infix "≡[ s ]≡" := (overlap s) (at level 70).
+
+  Record task_data :=
+    TaskData {
+        td_expr: expr;
+        td_env: env;
+        td_pre: types.heap;
+        td_post: types.heap;
+        td_D_pre: conn_map;
+        td_D_name: gname;
+        td_N_name: gname
+      }.
+  Canonical Structure task_dataC := leibnizC task_data.
+  Canonical Structure conn_mapC := leibnizC conn_map.
+  Canonical Structure name_mapC := leibnizC name_map.
+  Class taskDataG Σ :=
+    { td_taskData_inG:> inG Σ (agreeR task_dataC);
+      td_connData_inG:> inG Σ (oneshotR conn_mapC);
+      td_nameData_inG:> inG Σ (oneshotR name_mapC) }.
+  
+  (** First, define functions for each case separately. *)
+  Section TypeInterpretation.
+    Context `{implStateG Σ, specStateG Σ, axiomaticIrisG Σ, taskDataG Σ} (c0: cfg).
+
+    Local Open Scope I.
+    Definition intΓ (iτ: type → int_type) (Γ: env) (D: conn_map) (N: name_map)
+               (σ: gmap string val): iProp Σ :=
+      ⌜∀ x: string, is_Some (Γ !! x) ↔ is_Some (σ !! x)⌝ ∧
+            ⌜∀ x: string, is_Some (Γ !! x) ↔ is_Some (D !! var x)⌝ ∧
+                          ∀ (x: string) τ v d, ⌜Γ !! x = Some τ ∧
+                                               σ !! x = Some v ∧
+                                               D !! var x = Some d⌝ → iτ τ d N v.
+    Definition not_new (Γ: env) (η: types.heap) (τ: type) (η': types.heap): coPset :=
+      of_gset (names Γ ∪ names η) ∖ of_gset (names τ ∪ names η').
+
+    Definition simulation' iτ iτ' (iη iη': types.heap → int_heap) Γ e η τ η' D D': iProp Σ :=
+      ∀ N σ, existential_triple ⊤ c0
+                                (intΓ iτ Γ D N σ ∗ iη η D N)
+                                (subst (of_val <$> σ) e)
+                                (λ v, ∃ d N',
+                                    ⌜N ≡[not_new Γ η τ η']≡ N' ∧ D' !! RET = Some d⌝ ∧
+                                    iτ' τ d N' v ∗ iη' η' D' N').
+    
+    Implicit Type d : val.
+    Implicit Type N: name_map.
+    Implicit Type x: val.
+
+    Definition int_i_bool d N x: iProp Σ := ⌜(x = Ctrue ∨ x = Cfalse) ∧ x = d⌝.
+    Definition int_s_bool := int_i_bool.
+    Definition int_i_unit d N x: iProp Σ := ⌜x = Cunit⌝.
+    Definition int_s_unit := int_i_unit.
+    Definition int_i_ref (ξ: gname) d N x: iProp Σ := ⌜∃ l: loc, N!!ξ = Some (Loc l) ∧ x = Cloc l⌝.
+    Definition int_s_ref := int_i_ref.
+    Definition int_s_promise ξ d N x: iProp Σ := ⌜∃ t γ, N!!ξ = Some (Task t γ) ∧ x = Ctid t⌝.
+
+    (** We build the implementation interpretation of promise in stages. *)
+    (** Access to the task data. *)
+    Definition ip_data γ U (D': conn_map) (N': name_map) :=
+      own γ (to_agree U) ∗ own (td_D_name U) (agreed D') ∗ own (td_N_name U) (agreed N').
+    (** The easy parts: name map and implementation interpretation. *)
+    Definition ip_impl (A: gset gname) (τ: type) (τi: @int_type Σ) (D': conn_map) N' N y :=
+      ∃ d, ⌜D' !! RET = Some d ∧ N ≡[ of_gset (names τ) ∖ of_gset A ]≡ N'⌝ ∗ τi d N' y.
+    (** The simuation triple. Note that we have a bit of trouble here: As given in the
+        paper, the construction is not neccesarily well-founded. The complications with
+        the different its and so on are here to allow us to build a well-founded fixpoint
+        later on. *)
+    Definition ip_sim iτs iτs' iηs iηs' τ U D' :=
+      simulation' iτs iτs' iηs iηs' (td_env U) (td_expr U) (td_pre U) τ (td_post U) (td_D_pre U) D'.
+    (** Now, note that we only need to make our fixpoint well-founded for the
+        preconditions: τ is known to be structurally smaller, and the interpretation
+        of types does not recurse into that of heaps, so we can simply use the
+        same-level functions for the postconditions. But the names in the preconditions
+        will never be in allocation sets, so we can treat them as constant - in other
+        words, we can look up the task ids of all the ξ in the precondition! This allows
+        us to write down a description of type depth (i.e., how long a chain of promises
+        it induces). 
+        us to get the levels for those tasks, and formulate an invariant. *)
+    Fixpoint ty_all_tasks (ϕ: gname → iProp Σ) τ :=
+      match τ return iProp Σ with
+      | ttask ξ _ τ => ϕ ξ ∗ ty_all_tasks ϕ τ
+      | tref _ | tunit | tbool => True
+      end.
+    Fixpoint he_all_tasks (ϕ: gname → iProp Σ) η :=
+      match η return iProp Σ with
+      | hwait ξ _ η => ϕ ξ ∗ he_all_tasks ϕ η
+      | hstar η η' => he_all_tasks ϕ η ∗ he_all_tasks ϕ η'
+      | hpt _ _ | hemp => True
+      end.
+    Definition env_all_tasks ϕ (Γ: env) := ∀ (x: string) τ, ⌜Γ !! x = Some τ⌝ → ty_all_tasks ϕ τ.
+    Fixpoint depth N n γ {struct n} :=
+      match n return iProp Σ with
+      | O => False
+      | S n => ∀ γ (U: task_data),
+          own γ (to_agree U) -∗
+                     let ϕ ξ := (∀ p γ, ⌜N !! ξ = Some (Task p γ)⌝ → depth N n γ)
+                     in env_all_tasks ϕ (td_env U) ∗ he_all_tasks ϕ (td_pre U)
+      end.
+    (** Put together the inner pieces of the interpretation of promises... *)
+    Definition promiseN := nroot .@ "promise".
+    Definition int_i_promise_body iτs iτs' iηs iηs' N A τ τi γ v :=
+      ∀ U D' N',
+        ip_data γ U D' N' ∗ ip_impl A τ τi D' N' N v ∗ ip_sim iτs iτs' iηs iηs' τ U D'.
+    Definition int_i_promise iτs iτs' iηs iηs' ξ A τ τi d N x :=
+      ∃ t γ, ⌜N !! ξ = Some (Task t γ) ∧ x = Ctid t⌝ ∧
+           inv promiseN (wait t (int_i_promise_body iτs iτs' iηs iηs' N A τ τi γ)).
+  End TypeInterpretation.
+  Section HeapInterpretation.
+    Context `{implStateG Σ, specStateG Σ, axiomaticIrisG Σ, taskDataG Σ} (c0: cfg).
+    Implicit Type N : name_map.
+    Implicit Type D : conn_map.
+    Local Open Scope I.
+
+    Definition int_i_emp D N: iProp Σ := True.
+    Definition int_s_emp := int_i_emp.
+    Definition int_i_star (iη iη': int_heap) D N: iProp Σ := iη D N ∗ iη' D N.
+    Definition int_s_star := int_i_star.
+    Definition int_i_pt ξ (iτ: int_type) D N: iProp Σ :=
+      ∃ l d v, ⌜N!!ξ = Some (Loc l) ∧ D!!name ξ = Some d⌝ ∗ mapstoI l v 1%Qp ∗ iτ d N v.
+    Definition int_s_pt ξ (iτ: int_type) D N: iProp Σ :=
+      ∃ l d v, ⌜N!!ξ = Some (Loc l) ∧ D!!name ξ = Some d⌝ ∗ mapstoS l v 1%Qp ∗ iτ d N v.
+    Definition int_i_wait_body γ (η: types.heap) (iη: int_heap) A N :=
+      ∃ U D' N', ip_data γ U D' N' ∗ ⌜N ≡[ of_gset (names η) ∖ of_gset A]≡ N'⌝ ∗ iη D' N'.
+    Definition int_i_wait ξ A η (iη: int_heap) D N: iProp Σ :=
+      ∃ t γ, ⌜N!!ξ = Some (Task t γ)⌝ ∗ wait t (λ _, int_i_wait_body γ η iη A N).
+    (* Use the lower-level interpretations here *)
+    Definition int_s_wait_pre iτs' (iηs': types.heap → int_heap) U N' σ: iProp Σ :=
+      intΓ iτs' (td_env U) (td_D_pre U) N' σ ∗ iηs' (td_pre U) (td_D_pre U) N'.
+    Definition int_s_wait iτs' iηs' ξ A η D N :=
+      ∃ t γ U N' σ,
+        ⌜N!!ξ = Some (Task t γ) ∧ td_post U = η ∧ N ≡[of_gset (names η) ∖ of_gset A]≡ N'⌝ ∧
+        t ⤇ run: (subst (of_val <$> σ) (td_expr U)) ∗ int_s_wait_pre iτs' iηs' U N' σ.
+  End HeapInterpretation.
+
+  Section Interpretations.
+    Context `{implStateG Σ, specStateG Σ, axiomaticIrisG Σ, taskDataG Σ} (c0: cfg).
+    Implicit Type N: name_map.
+    Implicit Type D: conn_map.
+    Implicit Type x: val.
+    Implicit Type d: val.
+    Local Open Scope I.
+    
+    Fixpoint int_s_type τ: @int_type Σ :=
+      match τ with
+      | tbool => int_s_bool
+      | tunit => int_s_unit
+      | tref ξ => int_s_ref ξ
+      | ttask ξ A τ => int_s_promise ξ
+      end.
+    Fixpoint int_s_heap_approx iη η: @int_heap Σ :=
+      match η with
+      | hemp => int_s_emp
+      | hstar η η' => int_s_star (int_s_heap_approx iη η) (int_s_heap_approx iη η')
+      | hpt ξ τ => int_s_pt ξ (int_s_type τ)
+      | hwait ξ A η => int_s_wait int_s_type iη ξ A η
+      end.
+    Fixpoint int_s_heap_rec n η :=
+      match n return @int_heap Σ with
+      | O => int_s_heap_approx (λ _ _ _, False%I) η
+      | S n => int_s_heap_approx (int_s_heap_rec n) η
+      end.
+    Definition heap_depth N n η :=
+      he_all_tasks (λ ξ, ∀ t γ, ⌜N !! t = Some (Task t γ)⌝ → depth N n γ) η.
+    Definition int_s_heap η: @int_heap Σ := λ D N, ∃ n, heap_depth N n η ∗ int_s_heap_rec n η D N.
+
+    Fixpoint int_i_type τ: @int_type Σ :=
+      match τ with
+      | tbool => int_i_bool
+      | tunit => int_i_unit
+      | tref ξ => int_i_ref ξ
+      | ttask ξ A τ => int_i_promise c0 int_s_type int_s_type int_s_heap int_s_heap
+                                     ξ A τ (int_i_type τ)
+      end.
+    Fixpoint int_i_heap η: @int_heap Σ :=
+      match η with
+      | hemp => int_i_emp
+      | hstar η η' => int_i_star (int_i_heap η) (int_i_heap η')
+      | hpt ξ τ => int_i_pt ξ (int_i_type τ)
+      | hwait ξ A η => int_i_wait ξ A η (int_i_heap η)
+      end.
+
+    Definition int_s_env := intΓ int_s_type.
+    Definition int_i_env := intΓ int_i_type.
+    
+    (** Basic properties of interpretation *)
+    Global Instance int_s_type_persistent τ d N v:  PersistentP (int_s_type τ d N v).
+    Proof. destruct τ; apply _. Qed.
+    Global Instance int_i_type_persistent τ d N v:  PersistentP (int_i_type τ d N v).
+    Proof. destruct τ; apply _. Qed.
+    Global Instance int_s_env_persistent Γ D N σ: PersistentP (int_s_env Γ D N σ).
+    Proof. apply _. Qed.
+    Global Instance int_i_env_persistent Γ D N σ: PersistentP (int_i_env Γ D N σ).
+    Proof. apply _. Qed.
+
+    Lemma int_s_type_local τ: ∀ N N' d x (eqN: N ≡[names τ]≡ N'),
+        (int_s_type τ d N x ⊣⊢ int_s_type τ d N' x).
+    Proof.
+      induction τ; intros; cbn; try done.
+      - rewrite /int_s_ref /int_i_ref.
+        rewrite eqN; first done.
+        cbn; set_solver.
+      - rewrite /int_s_promise.
+        rewrite eqN; first done.
+        cbn -[union]; set_solver.
+    Qed.
+    Instance wait_proper t: Proper (pointwise_relation _ (≡) ==> (≡)) (@wait Σ t).
+    Proof.
+      intros ϕ ϕ' eqϕ.
+      rewrite equiv_dist; intro.
+      apply wait_nonexpansive; intro v.
+      rewrite eqϕ; done.
+    Qed.
+    
+    Lemma int_i_type_local τ: ∀ N N' d x (eqN: N ≡[names τ]≡ N'),
+        (int_i_type τ d N x ⊣⊢ int_i_type τ d N' x).
+    Proof.
+      induction τ; intros; cbn; try done.
+      - rewrite /int_i_ref eqN; first done.
+        cbn; set_solver.
+      - rewrite /int_i_promise.
+        f_equiv; intro t.
+        f_equiv; intro γ.
+        rewrite {1}eqN; last by (cbn -[union]; set_solver).
+        do 2 f_equiv.
+        rewrite /int_i_promise_body.
+        f_equiv; intro v.
+        f_equiv; intro U.
+        f_equiv; intro D'.
+        f_equiv; intro N''.
+        do 2 f_equiv.
+        rewrite /ip_impl.
+        f_equiv; intro d'.
+        do 3 f_equiv.
+        rewrite /overlap.
+        cbn -[union] in eqN.
+    Qed.
+
+    
+  End Interpretations.
+
+  (** Basic properties *)
+  Global Instance 
